Morph/Specs/ASTGraph/Examples.lean
@@ -1,5 +1,6 @@
 /- Copyright 2024-2025 The Morph Project Authors
 SPDX-License-Identifier: Apache-2.0
+-/
 
 
 import Morph.Specs.ASTGraph.Spec
