Morph/Specs/TypeSystem.lean
@@ -1,0 +1,6 @@
+/- Copyright 2024-2025 The Morph Project Authors
+SPDX-License-Identifier: Apache-2.0
+-/
+
+import Morph.Specs.TypeSystem.Spec
+import Morph.Specs.TypeSystem.Lemmas
