Morph/Specs/UnidirectionalDataFlow/Spec.lean
@@ -1,5 +1,6 @@
--- Copyright 2024-2025 The Morph Project Authors
--- SPDX-License-Identifier: Apache-2.0
+/- Copyright 2024-2025 The Morph Project Authors
+SPDX-License-Identifier: Apache-2.0
+-/
 
 import Morph.Core
 import Morph.Syntax
@@ -7,4 +8,9 @@ import Morph.Syntax
 namespace Morph.Specs.UnidirectionalDataFlow
 
 /-!
+# Unidirectional Data Flow Specification
+
+TODO: Implement this module.
 -/
+
+end Morph.Specs.UnidirectionalDataFlow
